Linglib.lean
@@ -1755,14 +1755,15 @@ import Linglib.Semantics.Modality.TemporalConstraint
 import Linglib.Semantics.Modality.Typology
 import Linglib.Semantics.Modification.Basic
 import Linglib.Semantics.Modification.RelativeClause
-import Linglib.Semantics.Mood.Basic
 import Linglib.Semantics.Mood.Categories
 import Linglib.Semantics.Mood.ClauseType
-import Linglib.Semantics.Mood.Dynamic
 import Linglib.Semantics.Mood.Component
+import Linglib.Semantics.Mood.Dynamic
+import Linglib.Semantics.Mood.Eventuality
 import Linglib.Semantics.Mood.Illocutionary
 import Linglib.Semantics.Mood.Modal
 import Linglib.Semantics.Mood.PartitionAsInquiry
+import Linglib.Semantics.Mood.Situation
 import Linglib.Semantics.Mood.State
 import Linglib.Semantics.Mood.Verbal
 import Linglib.Semantics.NaturalLogic
